例行提交. 2016/11/24. Kyo.

cpdt/ProofSeachByLP.v
@@ -95,3 +95,197 @@ info_eauto with slow.
 Qed.
 
 (* Chap13.2 *)
+Require Import List.
+
+Print length.
+
+Example length_1_2 :  length (1::2::nil)=2.
+auto. Qed.
+
+Print length_1_2.
+Theorem length_O : forall A, length (nil (A:=A))=O.
+  crush. Qed.
+Theorem length_S : forall A (h:A) t n,
+    length t=n -> length (h::t) = S n.
+  crush. Qed.
+Hint Resolve length_O length_S.
+
+Example length_is_2 : exists ls:list nat, length ls=2.
+eauto. Show Proof. Abort.
+
+Print Forall.
+Example length_is_2:  exists ls:list nat, length ls=2
+                                   /\ Forall (fun n=>n>=1) ls.
+eauto 9. Qed.
+Print length_is_2.
+Definition sum := fold_right plus O.
+
+Lemma plusO' : forall n m, n=m -> 0+n=m.
+  crush. Qed.
+
+Hint Resolve plusO'.
+Hint Extern 1 (sum _ = _) => simpl.
+
+Example length_and_sum : exists ls:list nat, length ls=2
+                                      /\ sum ls=O.
+eauto 7. Qed.
+
+Example length_and_sum' : exists ls:list nat, length ls=5 /\ sum ls=42.
+eauto 15. Qed.
+
+Example length_and_sum'' : exists ls: list nat, length ls=2
+                                         /\ sum ls=3
+                                         /\ Forall (fun n=> n<> 0) ls.
+eauto 11. Qed.
+
+(* chap13.3 *)
+Inductive exp:Set:=
+| Const:nat->exp
+| Var:exp
+| Plus : exp->exp ->exp.
+
+Inductive eval (var:nat) : exp->nat->Prop:=
+| EvalConst : forall n, eval var (Const n) n
+| EvalVar: eval var Var var
+| EvalPlus : forall e1 e2 n1 n2, eval var e1 n1->
+                            eval var e2 n2->
+                            eval var (Plus e1 e2) (n1+n2).
+Hint Constructors eval.
+
+Example eval1 : forall var, eval var (Plus Var (Plus (Const 8) Var)) (var + ( 8+var)).
+auto. Qed.
+Example eval1': forall var, eval var (Plus Var (Plus (Const 8) Var)) (2*var+8).
+eauto. Abort.
+
+Theorem EvalPlus' : forall var e1 e2 n1 n2 n, eval var e1 n1->
+                                         eval var e2 n2 ->
+                                         n1+n2=n->
+                                         eval var (Plus e1 e2) n.
+  crush. Qed.
+
+Hint Resolve EvalPlus'.
+
+Hint Extern 1 ( _ = _ ) => abstract omega.
+
+Example eval1': forall var, eval var (Plus Var (Plus (Const 8) Var)) (2*var+8).
+eauto. Qed.
+Print eval1'.
+
+Example synthesize1:exists e, forall var, eval var e (var +7).
+eauto. Qed.
+
+Print synthesize1.
+
+Example synthesize2:exists e,forall var, eval var e (2*var+8).
+eauto. Qed.
+Example synthesize3:exists e, forall var, eval var e (3*var+42).
+eauto. Qed.
+
+Theorem EvalConst' :forall var n m, n=m->
+                               eval var (Const n) m.
+  crush. Qed.
+Hint Resolve EvalConst'.
+
+Theorem zero_times : forall n m r, r=m->
+                              r=0*n+m.
+  crush. Qed.
+
+Hint Resolve zero_times.
+Theorem EvalVar' : forall var n, var=n ->eval var Var n.
+  crush. Qed.
+
+Hint Resolve EvalVar'.
+Theorem plus_0 : forall n r, r=n ->r = n+0.
+  crush. Qed.
+
+Theorem times_1 : forall n, n=1*n.
+  crush. Qed.
+Hint Resolve times_1 plus_0.
+
+Require Import Arith Ring.
+Theorem combine : forall x k1 k2 n1 n2,
+    (k1*x+n1)+(k2*x+n2)=(k1+k2)*x+(n1+n2).
+  intros; ring. Qed.
+
+Hint Resolve combine.
+Theorem linear : forall e, exists k, exists n, forall var, eval var e (k*var +n).
+  induction e; crush; eauto. Qed.
+
+(* 13.4 *)
+
+Theorem bool_neq : true <> false.
+  auto. Abort.
+Hint Extern 1 ( _ <> _) => congruence.
+
+Theorem bool_neq : true <> false.
+  auto. Qed.
+
+Section forall_and.
+  Variable A : Set.
+  Variables P Q:A->Prop.
+
+  Hypothesis both: forall x, P x /\ Q x.
+
+  Theorem forall_and : forall z, P z.
+    crush.
+    Hint Extern 1 (P ?X) =>
+    match goal with
+      | [ H:forall x, P x /\ _ |- _]=> apply (proj1 (H X))
+    end.
+    auto. Qed.
+
+End forall_and.
+  Hint Extern 1 =>
+  match goal with
+    | [ H: forall x, ?P x /\ _ |- ?P ?X]=> apply (proj1 (H X))
+  end.
+
+  (* 13.5 *)
+
+  Section autorewrite.
+    Variable A : Set.
+    Variable f : A->A.
+
+    Hypothesis f_f: forall x, f (f x)=f x.
+    Hint Rewrite f_f.
+    
+    Lemma f_f_f : forall x, f (f (f x))=f x.
+      intros; autorewrite with core; reflexivity. Qed.
+
+    Section garden_path.
+      Variable g : A->A.
+      Hypothesis f_g : forall x, f x=g x.
+
+      Hint Rewrite f_g.
+      Lemma f_f_f' : forall x, f (f (f x)) = f x.
+        intros; autorewrite with core. Abort.
+      Reset garden_path.
+      Section garden_path.
+        Variable P : A->Prop.
+        Variable g : A->A.
+
+        Hypothesis f_g : forall x, P x->f x=g x.
+        Hint Rewrite f_g.
+
+        Lemma f_f_f' : forall x, f (f (f x))=f x.
+          intros; autorewrite with core. Abort.
+
+        Reset garden_path.
+      Section garden_path.
+        Variable P : A->Prop.
+        Variable g : A->A.
+
+        Hypothesis f_g : forall x, P x->f x=g x.
+        Hint Rewrite f_g using assumption.
+
+        Lemma f_f_f' : forall x, f (f (f x))=f x.
+          intros; autorewrite with core; reflexivity. Qed.
+
+        Lemma f_f_f_g : forall x, P x->f (f x)=g x.
+          intros; autorewrite with core; reflexivity. Qed.
+      End garden_path.
+
+      Hint Rewrite f_f_f_g using assumption.
+      Lemma in_star : forall x y, f (f (f (f x)))=f (f y).
+        intros; autorewrite with core in *. Abort. 
+  End autorewrite.
