coq_summer_school/session9.v
@@ -1,0 +1,36 @@
+Require Import ZArith.
+Require Import Arith.
+
+Set Implicit Arguments.
+Set Asymmetric Patterns.
+
+Definition pred_safe : forall x, x<>0 -> nat.
+Inductive bnat (n:nat) : Type :=
+  cb : forall m , m<n ->bnat n.
+Inductive array (n:nat) : Type:=
+  ca: forall l:list Z, length l =n -> array n.
+
+Reset bnat.
+Definition bnat n := { m | m<n}.
+Definition array n := {l:list Z|length l =n}.
+Inductive sig (A:Type) (P:A->Prop) : Type := exist: forall x:A, P x-> sig P.
+(*
+Definition bsucc n:bnat n->bnat (S n) :=
+  fun m => let (x,p) := m in
+         exist _ (S x) (lt_n_S _ _ p).
+ *)
+Definition bsucc n:bnat n->bnat (S n).
+Proof. intros. destruct H.
+   exists (S x).
+   auto with arith. Qed. Abort.
+
+Section Test.
+  Reset sig. 
+  Inductive sig (A:Set) (P:A->Prop) : Set:=
+    exist : forall x:A, P x-> sig P.
+  Variable div_pair : forall a b:nat, 0<b ->
+                               {p:nat*nat | a=(fst p)*b+(snd p) /\ 0<=snd p <b}.
+  Implicit Arguments sig [A].
+
+
+End Test.
