tac/fresh.v
@@ -1,0 +1,8 @@
+Theorem t5 : (forall x:nat, S x> x)-> 2>1.
+  intros.
+  let H':=fresh "H'" in generalize H.
+  intros H'. auto. Qed.
+
+Theorem t5' : (forall x:nat, S x>x ) -> 2>1.
+  intros H.
+  let H':=fresh "H" in apply (H' 1). Qed.
